src/Verify.v
@@ -1,0 +1,143 @@
+Require Import LinearScan.Lib.
+Require Import Hask.Control.Monad.Trans.State.
+Require Import LinearScan.Context.
+Require Import LinearScan.UsePos.
+Require Import LinearScan.Interval.
+Require Import LinearScan.Blocks.
+Require Import LinearScan.ScanState.
+Require Import LinearScan.Morph.
+Require Import LinearScan.Cursor.
+Require Import LinearScan.Spec.
+Require Import LinearScan.Spill.
+Require Import LinearScan.Split.
+
+Set Implicit Arguments.
+Unset Strict Implicit.
+Unset Printing Implicit Defensive.
+Generalizable All Variables.
+
+Section Verify.
+
+Variable maxReg : nat.          (* max number of registers *)
+Definition PhysReg := 'I_maxReg.
+
+Variable maxVar : nat.          (* max number of variables *)
+Variables opType1 opType2 : Set.
+Variables mType : Type -> Type.
+Context `{mDict : Monad mType}.
+
+Variable oinfo : OpInfo maxReg opType1 opType2.
+
+Record RegStateDesc := {
+  rsRegs   : Vec (option 'I_maxVar) maxReg;
+  rsAllocs : Vec (option 'I_maxReg) maxVar;
+  rsStack  : Vec bool maxVar
+}.
+
+Definition newRegStateDesc : RegStateDesc :=
+  {| rsRegs   := vconst None
+   ; rsAllocs := vconst None
+   ; rsStack  := vconst false
+   |}.
+
+Definition IntSet_to_seq_fin {n : nat} (s : IntSet) :
+  all (ltn ^~ n) (IntSet_toList s) -> seq 'I_n.
+Proof.
+  elim: (IntSet_toList s) => [|x xs IHxs] /= H.
+    exact: [::].
+  move/andP: H => [H1 H2].
+  exact: cons (Ordinal H1) (IHxs _).
+Defined.
+
+Definition RV := ('I_maxReg + 'I_maxVar)%type.
+
+Inductive RegState : RegStateDesc -> Prop :=
+  | StartState : RegState newRegStateDesc
+
+  (* Based on the code flow analysis, [ins] is the set of incoming registers.
+     Anything other than these should not be presently active, all them should
+     be active, and they should apply to the correct variables. *)
+  | BeginBlock st ins :
+    forall H : all (ltn ^~ maxVar) (IntSet_toList ins),
+    all (fun var =>
+           if vnth (rsAllocs st) var isn't Some reg  then false else
+           if vnth (rsRegs st)   reg isn't Some var' then false else
+           var == var') (IntSet_to_seq_fin H) ->
+    RegState
+      {| rsRegs   := rsRegs st
+       ; rsAllocs := rsAllocs st
+       ; rsStack  := rsStack st
+       |}
+
+  | EndBlock st :
+    RegState
+      {| rsRegs   := rsRegs st
+       ; rsAllocs := rsAllocs st
+       ; rsStack  := rsStack st
+       |}
+
+  | AllocReg st r v :
+    RegState
+      {| rsRegs   := vreplace (rsRegs st) r (Some v)
+       ; rsAllocs := rsAllocs st
+       ; rsStack  := rsStack st
+       |}
+
+  | MoveReg st :
+    RegState
+      {| rsRegs   := rsRegs st
+       ; rsAllocs := rsAllocs st
+       ; rsStack  := rsStack st
+       |}
+
+  | SwapReg st :
+    RegState
+      {| rsRegs   := rsRegs st
+       ; rsAllocs := rsAllocs st
+       ; rsStack  := rsStack st
+       |}
+
+  | SpillReg st :
+    RegState
+      {| rsRegs   := rsRegs st
+       ; rsAllocs := rsAllocs st
+       ; rsStack  := rsStack st
+       |}
+
+  | RestoreReg st :
+    RegState
+      {| rsRegs   := rsRegs st
+       ; rsAllocs := rsAllocs st
+       ; rsStack  := rsStack st
+       |}
+
+  | FreeReg st :
+    RegState
+      {| rsRegs   := rsRegs st
+       ; rsAllocs := rsAllocs st
+       ; rsStack  := rsStack st
+       |}
+
+  | UseReg st :
+    RegState
+      {| rsRegs   := rsRegs st
+       ; rsAllocs := rsAllocs st
+       ; rsStack  := rsStack st
+       |}
+
+  | SetReg st :
+    RegState
+      {| rsRegs   := rsRegs st
+       ; rsAllocs := rsAllocs st
+       ; rsStack  := rsStack st
+       |}.
+
+Variable A : Type.
+
+Definition Verified := StateT { d : RegStateDesc * A | RegState (fst d) } mType.
+
+Definition verifyApplyAllocs (op : opType1) (allocs : seq (VarId * PhysReg)) :
+  Verified (seq opType2) :=
+  lift $ iso_to $ applyAllocs oinfo op allocs.
+
+End Verify.
